Impl/InsertModel.i.dfy
@@ -5,8 +5,6 @@ include "BookkeepingModel.i.dfy"
 include "FlushPolicyModel.i.dfy"
 
 module InsertModel { 
-  import opened StateSectorModel
-
   import opened IOModel
   import opened BookkeepingModel
   import opened FlushPolicyModel
